Replace CrashTolerant Forgotten nonsense with FloatingSeq

Spec/CrashTolerant.s.dfy
@@ -1,3 +1,4 @@
+include "../lib/Base/FloatingSeq.s.dfy"
 include "../lib/Base/SequencesLite.s.dfy"
 include "../lib/Base/MapRemove.s.dfy"
 include "RefinementObligation.s.dfy"
@@ -25,6 +26,7 @@ module CrashTolerantUIOp(atomic: AtomicStateMachineMod) refines UIOpIfc {
 
 module CrashTolerantMod(atomic: AtomicStateMachineMod) refines StateMachineIfc(CrashTolerantUIOp(atomic)) {
   import opened MapRemove_s
+  import opened FloatingSeqMod
   import opened SequencesLite // Last, DropLast
 
   // Crash tolerance adds asynchrony whether you like it or not.
@@ -39,55 +41,41 @@ module CrashTolerantMod(atomic: AtomicStateMachineMod) refines StateMachineIfc(C
   //import async = uiopifc.async
   //import async = StateMachineIfc(CrashTolerantUIOp(atomic)).uiopifc.async
 
-  // TODO(jonh): Use FloatingSeq developed with Jialin here!
-  datatype Version =
-    | Forgotten
-      // Keeping placeholders for LSNs before stableIdx makes it more
-      // obvious how the versions sequence evolves. To avoid the need
-      // for a bunch of ghost history complexity, we Forget the values
-      // at those LSNs so the implementation has an easy time constructing
-      // the interpretation.
-    | Version(asyncState: uiopifc.async.PersistentState)
-
   datatype Constants = Constants
+  type Version = uiopifc.async.PersistentState
   datatype Variables = Variables(
-    versions: seq<Version>,
+    versions: FloatingSeq<Version>,
     asyncEphemeral: uiopifc.async.EphemeralState,
 
     // Request id points at the number of LSNs that must be persisted.
     // So if the client ReqSyncs after 3 writes (seqEnd==3), the value
     // in the map is 3.
-    syncRequests: map<uiopifc.SyncReqId, nat>,
-
-    // TODO(jonh): reorder stableIdx aftern versions
-    // The index of the last persistent version. Notice that, since we
-    // never delete versions, that index is also the count of writes
-    // and thus also the "NextLSN" value when that version was created.
-    stableIdx: nat)
+    syncRequests: map<uiopifc.SyncReqId, nat>
+    )
   {
     predicate WF() {
       // There is always some persistent version, even if just a view of the
       // mkfs state
       && 0 < |versions|
+      && versions.IsActive(|versions|-1) // At least one active version
+    }
 
-      // All versions beginning with the stableIdx aren't truncated,
-      // so that crashing can't take us to a Forgotten version.
-      && (forall i | stableIdx<=i<|versions| :: versions[i].Version?)
-
-      && stableIdx < |versions|
+    // The stable index of the system; all later versions are liable to be lost on Crash
+    function StableIndex() : nat
+    {
+      versions.FirstActiveIndex()
     }
   }
 
-
   function InitState() : Variables {
-    Variables([Version(uiopifc.async.InitPersistentState())], uiopifc.async.InitEphemeralState(), map[], 0)
+    Variables(FloatingSeq(0, [uiopifc.async.InitPersistentState()]), uiopifc.async.InitEphemeralState(), map[])
   }
 
   // This isn't a transition, just a partial action for readibility.
-  predicate OptionallyAppendVersion(versions: seq<Version>, versions': seq<Version>)
+  predicate OptionallyAppendVersion(versions: FloatingSeq<Version>, versions': FloatingSeq<Version>)
   {
     // new versions list is either some new thing appended to the old one,
-    || (0<|versions'| && DropLast(versions') == versions)
+    || (0<|versions'| && versions'.DropLast() == versions)
     // or unchanged. We allow unchanged in the trusted spec so that
     // implementations don't have to account for number of read-only (query) ops.
     || versions' == versions
@@ -105,8 +93,8 @@ module CrashTolerantMod(atomic: AtomicStateMachineMod) refines StateMachineIfc(C
     && v'.WF()
     && OptionallyAppendVersion(v.versions, newVersions)
     && uiopifc.async.NextStep(
-        uiopifc.async.Variables(Last(v.versions).asyncState, v.asyncEphemeral),
-        uiopifc.async.Variables(Last(newVersions).asyncState, newAsyncEphemeral),
+        uiopifc.async.Variables(v.versions.Last(), v.asyncEphemeral),
+        uiopifc.async.Variables(newVersions.Last(), newAsyncEphemeral),
         op)
     && v' == v.(
         versions := newVersions,
@@ -120,7 +108,7 @@ module CrashTolerantMod(atomic: AtomicStateMachineMod) refines StateMachineIfc(C
   {
     && v.WF()
     && v' == v.(
-        versions := v.versions[..v.stableIdx+1],
+        versions := v.versions.GetPrefix(v.StableIndex()+1),
       // Crash forgets ephemeral stuff -- requests and syncRequests submitted but not answered.
         asyncEphemeral := uiopifc.async.InitEphemeralState(),
         syncRequests := map[]
@@ -137,15 +125,12 @@ module CrashTolerantMod(atomic: AtomicStateMachineMod) refines StateMachineIfc(C
     // let nondeterminism of v' choose this value
     // This wouldn't take so much explaining if we just exists newStableIdx, but then
     // it's harder to use and muddies up the UIOp skolem. Sorry.
-    && var newStableIdx := v'.stableIdx;
+    && var newStableIdx := v'.StableIndex();
 
     && v.WF()
-    && v.stableIdx <= newStableIdx < |v.versions|
-    && v' == v.(
-        // Commit forgets old versions.
-        versions := seq(|v.versions|, i requires 0<=i<|v.versions| =>
-          if i < newStableIdx then Forgotten else v.versions[i]),
-        stableIdx := newStableIdx)
+    && v.StableIndex() <= newStableIdx < |v.versions|
+    // Commit forgets old versions.
+    && v' == v.(versions := v.versions.GetSuffix(newStableIdx))
   }
 
   // sync api contract to the end user
@@ -166,7 +151,7 @@ module CrashTolerantMod(atomic: AtomicStateMachineMod) refines StateMachineIfc(C
   {
     && v.WF()
     && syncReqId in v.syncRequests
-    && v.syncRequests[syncReqId] <= v.stableIdx
+    && v.syncRequests[syncReqId] <= v.StableIndex()
     && v' == v.(syncRequests := MapRemove1(v.syncRequests, syncReqId))
   }
 
